src/Language/PlutusIR/Semantics/Static/Rules.v
@@ -1,166 +1,196 @@
-
 Require Import PlutusCert.Language.PlutusIR.
 Import NamedTerm.
 
+Require Export PlutusCert.Language.PlutusIR.Semantics.Static.Auxiliary.
+Require Export PlutusCert.Language.PlutusIR.Semantics.Static.Context.
+Require Export PlutusCert.Language.PlutusIR.Semantics.Static.Kinding.
+Require Export PlutusCert.Language.PlutusIR.Semantics.Static.Normalisation.
+Require Export PlutusCert.Language.PlutusIR.Semantics.Static.TypeSubstitution.
+
 Import Coq.Lists.List.
 Import Coq.Strings.String.
+Local Open Scope string_scope.
 
-Require Export PlutusCert.Language.PlutusIR.Semantics.Static.Implementations.
-Require Export PlutusCert.Language.PlutusIR.Semantics.Static.Normalisation.
+(** Types of builtin functions *)
+Definition lookupBuiltinTy (f : DefaultFun) : Ty :=
+  let Ty_Int := Ty_Builtin (Some (TypeIn DefaultUniInteger)) in
+  let Ty_Bool := Ty_Builtin (Some (TypeIn DefaultUniBool)) in
+  let Ty_BS := Ty_Builtin (Some (TypeIn DefaultUniByteString)) in
+  let T_Int_Bin := Ty_Fun Ty_Int (Ty_Fun Ty_Int Ty_Int) in
+  let T_Int_BinPredicate := Ty_Fun Ty_Int (Ty_Fun Ty_Int Ty_Bool) in
+  let T_BS_Bin := Ty_Fun Ty_BS (Ty_Fun Ty_BS Ty_BS) in
+  let T_BS_BinPredicate := Ty_Fun Ty_BS (Ty_Fun Ty_BS Ty_Bool) in
+  let Ty_Char := Ty_Builtin (Some (TypeIn DefaultUniChar)) in
+  let Ty_String := Ty_Builtin (Some (TypeIn DefaultUniString)) in
+  let Ty_Unit := Ty_Builtin (Some (TypeIn DefaultUniUnit)) in
+  match f with
+  | AddInteger => T_Int_Bin
+  | SubtractInteger => T_Int_Bin
+  | MultiplyInteger => T_Int_Bin
+  | DivideInteger => T_Int_Bin
+  | QuotientInteger => T_Int_Bin
+  | RemainderInteger => T_Int_Bin
+  | ModInteger => T_Int_Bin
+  | LessThanInteger => T_Int_BinPredicate
+  | LessThanEqInteger => T_Int_BinPredicate
+  | GreaterThanInteger => T_Int_BinPredicate
+  | GreaterThanEqInteger => T_Int_BinPredicate
+  | EqInteger => T_Int_BinPredicate
+  | Concatenate => T_BS_Bin
+  | TakeByteString => Ty_Fun Ty_Int (Ty_Fun Ty_BS Ty_BS)
+  | DropByteString => Ty_Fun Ty_Int (Ty_Fun Ty_BS Ty_BS)
+  | SHA2 => Ty_Fun Ty_BS Ty_BS
+  | SHA3 => Ty_Fun Ty_BS Ty_BS
+  | VerifySignature => Ty_Fun Ty_BS (Ty_Fun Ty_BS (Ty_Fun Ty_BS Ty_Bool))
+  | EqByteString => T_BS_BinPredicate
+  | LtByteString => T_BS_BinPredicate
+  | GtByteString => T_BS_BinPredicate
+  | IfThenElse => Ty_Forall "a" Kind_Base (Ty_Fun Ty_Bool (Ty_Fun (Ty_Var "a") (Ty_Fun (Ty_Var "a") (Ty_Var "a"))))
+  | CharToString => Ty_Fun Ty_Char Ty_String
+  | Append => Ty_Fun Ty_String (Ty_Fun Ty_String Ty_String)
+  | Trace => Ty_Fun Ty_String Ty_Unit (* TODO: figure out if it is the correct type*)
+  end.
 
-Create HintDb typing.
+(** Helper funcitons*)
+Definition flatten {A : Type} (l : list (list A)) := List.concat (rev l).
 
-(** ** Kinding of types *)
-Reserved Notation "Delta '|-*' ty ':' K" (at level 40, ty at level 0, K at level 0).
-Inductive has_kind : Delta -> Ty -> Kind -> Prop :=
-  | K_Var : forall Delta X K,
-      Delta X = Coq.Init.Datatypes.Some K ->
-      Delta |-* (Ty_Var X) : K
-  | K_Fun : forall Delta T1 T2,
+Fixpoint splitTy (T : Ty) : list Ty * Ty :=
+  match T with
+  | Ty_Fun Targ T' => (cons Targ (fst (splitTy T')), snd (splitTy T'))
+  | Tr => (nil, Tr)
+  end.
+
+Definition fromDecl (tvd : tvdecl tyname) : tyname * Kind :=
+  match tvd with
+  | TyVarDecl v K => (v, K)   
+  end.
+    
+Definition unwrapIFix (F : Ty) (K : Kind) (T : Ty) : Ty := (Ty_App (Ty_App F (Ty_Lam "X" K (Ty_IFix F (Ty_Var "X")))) T).
+
+(** Typing of terms *)
+Reserved Notation "Delta ',,' Gamma '[' flag ']|-+' t ':' T" (at level 101, flag at level 0, t at level 0, T at level 0, no associativity).
+Reserved Notation "Delta '|-ok_c' c ':' T" (at level 101, c at level 0, T at level 0).
+Reserved Notation "Delta ',,' Gamma '[' flag ']|-oks_nr' bs" (at level 101, flag at level 0, bs at level 0, no associativity).
+Reserved Notation "Delta ',,' Gamma '[' flag ']|-oks_r' bs" (at level 101, flag at level 0, bs at level 0, no associativity).
+Reserved Notation "Delta ',,' Gamma '[' flag ']|-ok_b' b" (at level 101, flag at level 0, b at level 0, no associativity).
+
+Inductive TypingFlag : Prop := | Escape | NoEscape .
+
+Inductive has_type : TypingFlag -> Delta -> Gamma -> Term -> Ty -> Prop :=
+  (* Simply typed lambda caclulus *)
+  | T_Var : forall Gamma Delta x T Tn flag,
+      Gamma x = Coq.Init.Datatypes.Some T ->
+      normalise T Tn ->
+      Delta ,, Gamma [ flag ]|-+ (Var x) : Tn
+  | T_LamAbs : forall Delta Gamma x T1 t T2n T1n flag,
       Delta |-* T1 : Kind_Base ->
-      Delta |-* T2 : Kind_Base ->
-      Delta |-* (Ty_Fun T1 T2) : Kind_Base
-  | K_IFix  : forall Delta F T K,
+      normalise T1 T1n ->
+      Delta ,, x |-> T1n; Gamma [ flag ]|-+ t : T2n -> 
+      Delta ,, Gamma [ flag ]|-+ (LamAbs x T1 t) : (Ty_Fun T1n T2n)
+  | T_Apply : forall Delta Gamma t1 t2 T1n T2n flag,
+      Delta ,, Gamma [ flag ]|-+ t1 : (Ty_Fun T1n T2n) ->
+      Delta ,, Gamma [ flag ]|-+ t2 : T1n ->
+      Delta ,, Gamma [ flag ]|-+ (Apply t1 t2) : T2n
+  (* Universal quantification*)
+  | T_TyAbs : forall Delta Gamma X K t Tn flag,
+      (X |-> K; Delta) ,, Gamma [ flag ]|-+ t : Tn ->
+      Delta ,, Gamma [ flag ]|-+ (TyAbs X K t) : (Ty_Forall X K Tn)
+  | T_TyInst : forall Delta Gamma t1 T2 T1n X K2 T0n T2n flag,
+      Delta ,, Gamma [ flag ]|-+ t1 : (Ty_Forall X K2 T1n) ->
+      Delta |-* T2 : K2 ->
+      normalise T2 T2n ->
+      normalise (substituteTCA X T2n T1n) T0n ->
+      Delta ,, Gamma [ flag ]|-+ (TyInst t1 T2) : T0n
+  (* Recursive types *)
+  | T_IWrap : forall Delta Gamma F T M K Tn Fn T0n flag,
       Delta |-* T : K ->
+      normalise T Tn ->
       Delta |-* F : (Kind_Arrow (Kind_Arrow K Kind_Base) (Kind_Arrow K Kind_Base)) ->
-      Delta |-* (Ty_IFix F T) : Kind_Base
-  | K_Forall : forall Delta X K T,
-      (X |-> K; Delta) |-* T : Kind_Base ->
-      Delta |-* (Ty_Forall X K T) : Kind_Base
-  | K_Builtin : forall Delta u T,
-      T = lookupBuiltinKind u ->
-      Delta |-* (Ty_Builtin (Some (TypeIn u))) : T
-  | K_Lam : forall Delta X K1 T K2,
-      (X |-> K1; Delta) |-* T : K2 ->
-      Delta |-* (Ty_Lam X K1 T) : (Kind_Arrow K1 K2)
-  | K_App : forall Delta T1 T2 K1 K2,
-      Delta |-* T1 : (Kind_Arrow K1 K2) ->
-      Delta |-* T2 : K1 ->
-      Delta |-* (Ty_App T1 T2) : K2
-where "Delta '|-*' ty ':' K" := (has_kind Delta ty K).
-
-(** ** Typing of terms *)
-Reserved Notation "Delta ',,' Gamma '|-+' t ':' T" (at level 101, t at level 0, T at level 0).
-
-Inductive has_type : Delta -> Gamma -> Term -> Ty -> Prop :=
+      normalise F Fn ->
+      normalise (unwrapIFix Fn K Tn) T0n ->
+      Delta ,, Gamma [ flag ]|-+ M : T0n ->
+      Delta ,, Gamma [ flag ]|-+ (IWrap F T M) : (Ty_IFix Fn Tn)
+  | T_Unwrap : forall Delta Gamma M Fn K Tn T0n flag,
+      Delta ,, Gamma [ flag ]|-+ M : (Ty_IFix Fn Tn) ->
+      Delta |-* Tn : K ->
+      normalise (unwrapIFix Fn K Tn) T0n ->
+      Delta ,, Gamma [ flag ]|-+ (Unwrap M) : T0n
+  (* Additional constructs *)
+  | T_Constant : forall Delta Gamma u a flag,
+      Delta ,, Gamma [ flag ]|-+ (Constant (Some (ValueOf u a))) : (Ty_Builtin (Some (TypeIn u)))
+  | T_Builtin : forall Delta Gamma f T Tn flag,
+      T = lookupBuiltinTy f ->
+      normalise T Tn ->
+      Delta ,, Gamma [ flag ]|-+ (Builtin f) : Tn
+  | T_Error : forall Delta Gamma S T Tn flag,
+      Delta |-* T : Kind_Base ->
+      normalise T Tn ->
+      Delta ,, Gamma [ flag ]|-+ (Error S) : Tn
   (** Let-bindings
       Note: The rules for let-constructs differ significantly from the paper definitions
       because we had to adapt the typing rules to the compiler implementation of type checking.
       Reference: The Haskell module Language.PlutusIR.TypeCheck.Internal in the 
       iohk/plutus/plutus-core/plutus-ir project.
   **)
-  | T_Let : forall Delta Gamma bs t Tn Delta' Gamma' bsGn,
+  | T_Let : forall Delta Gamma bs t Tn Delta' Gamma' bsGn flag,
       Delta' = mupdate Delta (flatten (map binds_Delta bs)) ->
       map_normalise (flatten (map binds_Gamma bs)) bsGn -> 
       Gamma' = mupdate Gamma bsGn ->
-      bindings_well_formed_nonrec Delta Gamma bs ->
-      Delta' ,, Gamma' |-+ t : Tn ->
-      Delta ,, Gamma |-+ (Let NonRec bs t) : Tn
-  | T_LetRec : forall Delta Gamma bs t Tn Delta' Gamma' bsGn,
+      Delta ,, Gamma [flag]|-oks_nr bs ->
+      Delta' ,, Gamma' [ flag ]|-+ t : Tn ->
+      (flag = NoEscape -> Delta |-* Tn : Kind_Base) ->
+      Delta ,, Gamma [ flag ]|-+ (Let NonRec bs t) : Tn
+  | T_LetRec : forall Delta Gamma bs t Tn Delta' Gamma' bsGn flag,
       Delta' = mupdate Delta (flatten (map binds_Delta bs)) ->
       map_normalise (flatten (map binds_Gamma bs)) bsGn -> 
       Gamma' = mupdate Gamma bsGn ->
-      bindings_well_formed_rec Delta' Gamma' bs ->
-      Delta' ,, Gamma' |-+ t : Tn ->
-      Delta ,, Gamma |-+ (Let Rec bs t) : Tn
-  (* Basic constructs *)
-  | T_Var : forall Gamma Delta x T Tn,
-      Gamma x = Coq.Init.Datatypes.Some T ->
-      normalise T Tn ->
-      Delta ,, Gamma |-+ (Var x) : Tn
-  | T_TyAbs : forall Delta Gamma X K t Tn,
-      (X |-> K; Delta) ,, Gamma |-+ t : Tn ->
-      Delta ,, Gamma |-+ (TyAbs X K t) : (Ty_Forall X K Tn)
-  | T_LamAbs : forall Delta Gamma x T1 t T2n T1n,
-      Delta |-* T1 : Kind_Base ->
-      normalise T1 T1n ->
-      Delta ,, x |-> T1n; Gamma |-+ t : T2n -> 
-      Delta ,, Gamma |-+ (LamAbs x T1 t) : (Ty_Fun T1n T2n)
-  | T_Apply : forall Delta Gamma t1 t2 T1n T2n,
-      Delta ,, Gamma |-+ t1 : (Ty_Fun T1n T2n) ->
-      Delta ,, Gamma |-+ t2 : T1n ->
-      Delta ,, Gamma |-+ (Apply t1 t2) : T2n
-  | T_Constant : forall Delta Gamma u a,
-      Delta ,, Gamma |-+ (Constant (Some (ValueOf u a))) : (Ty_Builtin (Some (TypeIn u)))
-  | T_Builtin : forall Delta Gamma f Tn,
-      Tn = lookupBuiltinTy f ->
-      Delta ,, Gamma |-+ (Builtin f) : Tn
-  | T_TyInst : forall Delta Gamma t1 T2 T1n X K2 T0n T2n,
-      Delta ,, Gamma |-+ t1 : (Ty_Forall X K2 T1n) ->
-      Delta |-* T2 : K2 ->
-      normalise T2 T2n ->
-      normalise (substituteTCA X T2n T1n) T0n ->
-      Delta ,, Gamma |-+ (TyInst t1 T2) : T0n
-  | T_Error : forall Delta Gamma T Tn,
-      Delta |-* T : Kind_Base ->
-      normalise T Tn ->
-      Delta ,, Gamma |-+ (Error T) : Tn
-  (* Recursive types *)
-  | T_IWrap : forall Delta Gamma F T M K T0n Tn Fn,
-      normalise (unwrapIFix F K T) T0n ->
-      Delta ,, Gamma |-+ M : T0n ->
-      Delta |-* T : K ->
-      normalise T Tn ->
-      Delta |-* F : (Kind_Arrow (Kind_Arrow K Kind_Base) (Kind_Arrow K Kind_Base)) ->
-      normalise F Fn ->
-      Delta ,, Gamma |-+ (IWrap F T M) : (Ty_IFix Fn Tn)
-  | T_Unwrap : forall Delta Gamma M Fn K Tn T0n,
-      Delta ,, Gamma |-+ M : (Ty_IFix Fn Tn) ->
-      Delta |-* Tn : K ->
-      normalise (unwrapIFix Fn K Tn) T0n ->
-      Delta ,, Gamma |-+ (Unwrap M) : T0n
+      Delta' ,, Gamma' [ flag ]|-oks_r bs ->
+      Delta' ,, Gamma' [ flag ]|-+ t : Tn ->
+      (flag = NoEscape -> Delta |-* Tn : Kind_Base) ->
+      Delta ,, Gamma [ flag ]|-+ (Let Rec bs t) : Tn
 
-  (* Extras *)
-  | T_ExtBuiltin : forall Delta Gamma f args Targs Tr Tr',
-      List.length args <= arity f ->
-      (Targs, Tr) = splitTy (lookupBuiltinTy f) ->
-      (forall p, In p (List.combine args Targs) -> Delta ,, Gamma |-+ (fst p) : (snd p)) ->
-      Tr' = combineTy (skipn (List.length args) Targs) Tr ->
-      Delta ,, Gamma |-+ (ExtBuiltin f args) : Tr'
-
-  with constructor_well_formed : Delta -> constructor -> Prop :=
+  with constructor_well_formed : Delta -> constructor -> Ty -> Prop :=
     | W_Con : forall Delta x T ar Targs Tr,
         (Targs, Tr) = splitTy T -> 
         (forall U, In U Targs -> Delta |-* U : Kind_Base) ->
-        constructor_well_formed Delta (Constructor (VarDecl x T) ar)
+        Delta |-ok_c (Constructor (VarDecl x T) ar) : Tr
 
-  with bindings_well_formed_nonrec : Delta -> Gamma -> list Binding -> Prop :=
-    | W_NilB_NonRec : forall Delta Gamma,
-        bindings_well_formed_nonrec Delta Gamma nil
-    | W_ConsB_NonRec : forall Delta Gamma b bs bsGn,
-        binding_well_formed Delta Gamma b ->
+  with bindings_well_formed_nonrec : TypingFlag -> Delta -> Gamma -> list Binding -> Prop :=
+    | W_NilB_NonRec : forall Delta Gamma flag,
+      Delta ,, Gamma [ flag ]|-oks_nr nil
+    | W_ConsB_NonRec : forall Delta Gamma b bs bsGn flag,
+        Delta ,, Gamma [ flag ]|-ok_b b ->
         map_normalise (binds_Gamma b) bsGn ->
-        bindings_well_formed_nonrec (mupdate Delta (binds_Delta b)) (mupdate Gamma bsGn) bs ->
-        bindings_well_formed_nonrec Delta Gamma (b :: bs)
+        (mupdate Delta (binds_Delta b)) ,, (mupdate Gamma bsGn) [ flag ]|-oks_nr bs ->
+        Delta ,, Gamma [ flag ]|-oks_nr (b :: bs)
 
-  with bindings_well_formed_rec : Delta -> Gamma -> list Binding -> Prop :=
-    | W_NilB_Rec : forall Delta Gamma,
-        bindings_well_formed_rec Delta Gamma nil
-    | W_ConsB_Rec : forall Delta Gamma b bs,
-        binding_well_formed Delta Gamma b ->
-        bindings_well_formed_rec Delta Gamma bs ->
-        bindings_well_formed_rec Delta Gamma (b :: bs)
+  with bindings_well_formed_rec : TypingFlag -> Delta -> Gamma -> list Binding -> Prop :=
+    | W_NilB_Rec : forall Delta Gamma flag,
+        Delta ,, Gamma [ flag ]|-oks_r nil
+    | W_ConsB_Rec : forall Delta Gamma b bs flag,
+        Delta ,, Gamma [ flag ]|-ok_b b ->
+        Delta ,, Gamma [ flag ]|-oks_r bs ->
+        Delta ,, Gamma [ flag ]|-oks_r (b :: bs)
 
-  with binding_well_formed : Delta -> Gamma -> Binding -> Prop :=
-    | W_Term : forall Delta Gamma s x T t,
+  with binding_well_formed : TypingFlag -> Delta -> Gamma -> Binding -> Prop :=
+    | W_Term : forall Delta Gamma s x T t Tn flag,
         Delta |-* T : Kind_Base ->
-        Delta ,, Gamma |-+ t : T ->
-        binding_well_formed Delta Gamma (TermBind s (VarDecl x T) t)
-    | W_Type : forall Delta Gamma X K T,
+        normalise T Tn ->
+        Delta ,, Gamma [ NoEscape ]|-+ t : Tn ->
+        Delta ,, Gamma [ flag ]|-ok_b (TermBind s (VarDecl x T) t)
+    | W_Type : forall Delta Gamma X K T flag,
         Delta |-* T : K ->
-        binding_well_formed Delta Gamma (TypeBind (TyVarDecl X K) T)
-    | W_Data : forall Delta Gamma X YKs cs matchFunc Delta' Gamma',
+        Delta ,, Gamma [ flag ]|-ok_b (TypeBind (TyVarDecl X K) T)
+    | W_Data : forall Delta Gamma X YKs cs matchFunc Delta' flag,
         Delta' = mupdate Delta (rev (map fromDecl YKs)) ->
-        Gamma' = Gamma ->
-        (forall c, In c cs -> constructor_well_formed Delta' c) ->
-        binding_well_formed Delta Gamma (DatatypeBind (Datatype X YKs matchFunc cs))
+        (forall c, In c cs -> Delta' |-ok_c c : (constrLastTy (Datatype X YKs matchFunc cs))) ->
+        Delta ,, Gamma [ flag ]|-ok_b (DatatypeBind (Datatype X YKs matchFunc cs))
 
-  where "Delta ',,' Gamma '|-+' t ':' T" := (has_type Delta Gamma t T).
-
-Notation "Delta '|-ok_c' c" := (constructor_well_formed Delta c) (at level 101, c at level 0).
-Notation "Delta ',,' Gamma '|-oks_nr' bs" := (bindings_well_formed_nonrec Delta Gamma bs) (at level 101, bs at level 0).
-Notation "Delta ',,' Gamma '|-oks_r' bs" := (bindings_well_formed_rec Delta Gamma bs) (at level 101, bs at level 0).
-Notation "Delta ',,' Gamma '|-ok' b" := (binding_well_formed Delta Gamma b) (at level 101, b at level 0).
+  where "Delta ',,' Gamma '[' flag ']|-+' t ':' T" := (has_type flag Delta Gamma t T)
+  and  "Delta '|-ok_c' c ':' T" := (constructor_well_formed Delta c T)
+  and "Delta ',,' Gamma '[' flag ']|-oks_nr' bs" := (bindings_well_formed_nonrec flag Delta Gamma bs)
+  and "Delta ',,' Gamma '[' flag ']|-oks_r' bs" := (bindings_well_formed_rec flag Delta Gamma bs)
+  and "Delta ',,' Gamma '[' flag ']|-ok_b' b" := (binding_well_formed flag Delta Gamma b).
 
 Scheme has_type__ind := Minimality for has_type Sort Prop
   with constructor_well_formed__ind := Minimality for constructor_well_formed Sort Prop
@@ -173,14 +203,6 @@ Combined Scheme has_type__multind from
   bindings_well_formed_nonrec__ind,
   bindings_well_formed_rec__ind,
   binding_well_formed__ind.
-
-#[export] Hint Constructors has_kind : typing.
-
-#[export] Hint Constructors has_type : typing.
-#[export] Hint Constructors constructor_well_formed : typing.
-#[export] Hint Constructors bindings_well_formed_nonrec : typing.
-#[export] Hint Constructors bindings_well_formed_rec : typing.
-#[export] Hint Constructors binding_well_formed : typing.
 
 Lemma strong_normalisation : forall Delta T K,
     Delta |-* T : K ->
@@ -202,35 +224,19 @@ Proof.
     inversion H; subst.
     + eauto.
     + destruct u; inversion H3.
-    + Axiom skip: forall P, P. apply skip.
+    + admit.
     + inversion H1; subst.
-      * apply skip.
+      * admit.
       * apply normalise_to_normal in H1 as Hnorm.
         inversion Hnorm; subst.
         eauto.
-Qed.
+Admitted.
 
-Lemma has_type__normal : forall Delta Gamma t T,
-    Delta ,, Gamma |-+ t : T ->
+Lemma has_type__normal : forall Delta Gamma flag t T,
+    Delta ,, Gamma [ flag ]|-+ t : T ->
     normal_Ty T.
 Proof with eauto.
-  induction 1; intros.
-  - assumption.
-  - assumption.
-  - eapply normalise_to_normal; eauto.
-  - eauto.
-  - eapply normalise_to_normal in H0...
+  induction 1; intros; eauto using normalise_to_normal...
   - inversion IHhas_type1; subst...
     inversion H1.
-  - eauto.
-  - destruct f; simpl in H; inversion H; subst...
-    apply NO_TyForall...
-    apply NO_TyFun...
-    apply NO_TyFun...
-  - eapply normalise_to_normal...
-  - eapply normalise_to_normal...
-  - eapply normalise_to_normal in H2...
-    eapply normalise_to_normal in H4...
-  - eapply normalise_to_normal...
-  - apply skip.
 Qed.
