src/Language/PlutusIR/Semantics/Static/Theorems/ContextInvariance.v
@@ -4,432 +4,139 @@ Import NamedTerm.
 Require Import PlutusCert.Language.PlutusIR.Semantics.Static.Theorems.ContextInvariance.AFI.
 Require Import PlutusCert.Language.PlutusIR.Semantics.Static.Rules.
 
-Require Import Coq.Logic.FunctionalExtensionality.
-Require Import Coq.Lists.List.
-Require Import PlutusCert.Util.
+Local Open Scope string_scope.
 
-(** * Context invariance *)
+Module Kinding.
 
-(** ** Type-level context invariance *)
-
-
-  
-
-
-(** *** Context invariance (Lemma) *)
-Lemma context_invariance__typelevel : forall Delta Delta' T K,
-    Delta |-* T : K ->
-    (forall X, appears_free_in_Ty X T -> Delta X = Delta' X) ->
-    Delta' |-* T : K.
-Proof with auto.
-  intros Delta Delta' T K HK.
-  generalize dependent Delta'.
-  induction HK; intros; try solve [econstructor; auto].
-  - apply K_Var.
-    rewrite <- H0...
-  - (* K_Forall *)
-    apply K_Forall.
-    apply IHHK.
-    intros.
-    destruct (X =? X0) eqn:Heqb.
-    + apply eqb_eq in Heqb.
-      subst.
-      rewrite update_eq.
-      rewrite update_eq.
-      reflexivity.
-    + apply eqb_neq in Heqb.
-      rewrite update_neq...
-      rewrite update_neq...
-  - (* K_Lam *)
-    apply K_Lam.
-    apply IHHK.
-    intros.
-    destruct (X =? X0) eqn:Heqb.
-    + apply eqb_eq in Heqb.
-      subst.
-      rewrite update_eq.
-      rewrite update_eq.
-      reflexivity.
-    + apply eqb_neq in Heqb.
-      rewrite update_neq...
-      rewrite update_neq...
-Qed.
-
-(** *** Free variables are in context (Lemma) *)
-
-Lemma free_in_context__Ty : forall X T K Delta,
-    appears_free_in_Ty X T ->
-    Delta |-* T : K ->
-    exists K', Delta X = Datatypes.Some K'.
-Proof with eauto.
-  intros X T K Delta Hafi Htyp.
-  induction Htyp; inversion Hafi; subst...
-  - rewrite update_neq in IHHtyp; auto.
-  - rewrite update_neq in IHHtyp; auto.
-Qed.
-
-Corollary typable_empty__closed_Ty : forall T K,
-    empty |-* T : K ->
-    closed_Ty T.
-Proof.
-  intros. unfold closed_Ty. intros x H1.
-  destruct (free_in_context__Ty _ _ _ _ H1 H) as [T' C].
-  discriminate C.
-Qed.
-
-(** ** Term-level context invariance *)
-
-
-
-(** ** Context invariance (Theorem) *)
-
-Definition P_has_type (Delta : Delta) (Gamma : Gamma) (t : Term) (T : Ty) :=
-  forall Gamma',
-    (forall x, appears_free_in_Term x t -> Gamma x = Gamma' x) ->
-    Delta ,, Gamma' |-+ t : T.
-
-Definition P_constructor_well_formed (Delta : Delta) (c : constructor) :=
-  Delta |-ok_c c.
-
-Definition P_bindings_well_formed_nonrec (Delta : Delta) (Gamma : Gamma) (bs : list Binding) :=
-  forall Gamma',
-    (forall x, appears_free_in_Term__bindings_nonrec x bs -> Gamma x = Gamma' x) ->
-    Delta ,, Gamma' |-oks_nr bs.  
-
-Definition P_bindings_well_formed_rec (Delta : Delta) (Gamma : Gamma) (bs : list Binding) :=
-  forall Gamma',
-    (forall x, appears_free_in_Term__bindings_rec x bs -> Gamma x = Gamma' x) ->
-    Delta ,, Gamma' |-oks_r bs.  
-
-Definition P_binding_well_formed (Delta : Delta) (Gamma : Gamma) (b : Binding) :=
-  forall Gamma',
-    (forall x, appears_free_in_Term__binding x b -> Gamma x = Gamma' x) ->
-    Delta ,, Gamma' |-ok b.
-
-#[export] Hint Unfold 
-  P_has_type
-  P_constructor_well_formed
-  P_bindings_well_formed_nonrec
-  P_bindings_well_formed_rec
-  P_binding_well_formed 
-  : core.
-
-Axiom skip : forall P, P.
-
-Theorem context_invariance : 
-  (forall Delta Gamma t T, Delta ,, Gamma |-+ t : T -> P_has_type Delta Gamma t T) /\
-  (forall Delta Gamma bs, Delta ,, Gamma |-oks_nr bs -> P_bindings_well_formed_nonrec Delta Gamma bs) /\
-  (forall Delta Gamma bs, Delta ,, Gamma |-oks_r bs -> P_bindings_well_formed_rec Delta Gamma bs) /\
-  (forall Delta Gamma b, Delta ,, Gamma |-ok b -> P_binding_well_formed Delta Gamma b).
-Proof with eauto.
-  apply has_type__multind with
-    (P := P_has_type)
-    (P0 := P_constructor_well_formed)
-    (P1 := P_bindings_well_formed_nonrec)
-    (P2 := P_bindings_well_formed_rec)
-    (P3 := P_binding_well_formed).
-  all: intros; autounfold; intros.
-  - (* T_Let *)
-    subst.
-    eapply T_Let.
-    + reflexivity.
-    + eassumption.
-    + reflexivity.
-    + apply H3.
+  Lemma context_invariance : forall Delta Delta' T K,
+      Delta |-* T : K ->
+      (forall X, Ty.appears_free_in X T -> Delta X = Delta' X) ->
+      Delta' |-* T : K.
+  Proof with auto.
+    intros Delta Delta' T K HK.
+    generalize dependent Delta'.
+    induction HK; intros; try solve [econstructor; eauto].
+    - apply K_Var.
+      rewrite <- H0...
+    - (* K_Forall *)
+      apply K_Forall.
+      apply IHHK.
       intros.
-      apply H6.
-      apply AFIT_LetNonRec.
-      assumption.
-    + simpl. apply H5.
-      intros.
-      apply mupdate_eq_cong.
-      apply H6.
-      apply AFIT_Let.
-      -- apply skip. (* TODO *) 
-      -- assumption.
-  - (* T_LetRec *)
-    subst.
-    eapply T_LetRec.
-    + reflexivity.
-    + eassumption.
-    + reflexivity.
-    + apply H3.
-      intros.
-      apply mupdate_eq_cong.
-      apply H6.
-      apply AFIT_LetRec; auto.
-      apply skip.
-    + apply H5.
-      intros.
-      apply mupdate_eq_cong.
-      apply H6.
-      apply AFIT_Let.
-      -- apply skip. (* TODO *)
-      -- assumption.
-  - (* T_Var *)
-    eapply T_Var...
-    rewrite <- H1; auto.
-  - (* T_TyForall *)
-    apply T_TyAbs.
-    apply H0.
-    intros x Hafi.
-    apply H1.
-    apply AFIT_TyAbs.
-    assumption.
-  - (* T_LamAbs *)
-    apply T_LamAbs.
-    + assumption.
-    + assumption.
-    + apply H2.
-      intros.
-      destruct (x =? x0) eqn:Heqb.
-      * apply eqb_eq in Heqb.
+      destruct (X =? X0) eqn:Heqb.
+      + apply eqb_eq in Heqb.
         subst.
         rewrite update_eq.
         rewrite update_eq.
         reflexivity.
-      * apply eqb_neq in Heqb.
-        rewrite update_neq; auto.
-        rewrite update_neq; auto.
-  - (* T_Apply *)
-    apply T_Apply with T1n.
-    + apply H0.
+      + apply eqb_neq in Heqb.
+        rewrite update_neq...
+        rewrite update_neq...
+    - (* K_Lam *)
+      apply K_Lam.
+      apply IHHK.
       intros.
-      apply H3.
-      apply AFIT_Apply1.
-      assumption.
-    + apply H2.
-      intros.
-      apply H3.
-      apply AFIT_Apply2.
-      assumption.
-  - (* T_Constant *)
-    apply T_Constant.
-  - (* T_Builtin *)
-    apply T_Builtin.
-    assumption.
-  - (* T_TyInst *)
-    apply T_TyInst with T1n X K2 T2n.
-    + apply H0.
-      intros.
-      apply H4.
-      apply AFIT_TyInst.
-      assumption.
-    + assumption.
-    + assumption.
-    + assumption.
-  - (* T_Error *)
-    apply T_Error.
-    assumption.
-    assumption.
-  - (* T_IWrap *)
-    apply T_IWrap with K T0n.
-    + assumption.
-    + apply H1.
-      intros.
-      apply H6.
-      apply AFIT_IWrap.
-      assumption.
-    + assumption.
-    + assumption.
-    + assumption.
-    + assumption.
-  - (* T_Unwrap *)
-    apply T_Unwrap with Fn K Tn.
-    + apply H0.
-      intros.
-      apply H3.
-      apply AFIT_Unwrap.
-      assumption.
-    + assumption.
-    + assumption.
+      destruct (X =? X0) eqn:Heqb.
+      + apply eqb_eq in Heqb.
+        subst.
+        rewrite update_eq.
+        rewrite update_eq.
+        reflexivity.
+      + apply eqb_neq in Heqb.
+        rewrite update_neq...
+        rewrite update_neq...
+  Qed.
 
-  - (* T_ExtBuiltin *)
-    eapply T_ExtBuiltin.
-    + eauto.
-    + eauto.
-    + intros.
-      eapply H2.
-      all: eauto.
-      destruct p.
-      simpl.
+End Kinding.
+
+Module Typing.
+
+  Definition P_has_type (flag : TypingFlag) (Delta : Delta) (Gamma : Gamma) (t : Term) (T : Ty) :=
+    forall Gamma',
+      (forall x, Term.appears_free_in x t -> Gamma x = Gamma' x) ->
+      Delta ,, Gamma' [ flag ]|-+ t : T.
+
+  Definition P_constructor_well_formed (Delta : Delta) (c : constructor) (T : Ty) :=
+    Delta |-ok_c c : T.
+
+  Definition P_bindings_well_formed_nonrec (flag : TypingFlag) (Delta : Delta) (Gamma : Gamma) (bs : list Binding) :=
+    forall Gamma',
+      (forall x, Term.appears_free_in__bindings_nonrec x bs -> Gamma x = Gamma' x) ->
+      Delta ,, Gamma' [ flag ]|-oks_nr bs.  
+
+  Definition P_bindings_well_formed_rec (flag : TypingFlag) (Delta : Delta) (Gamma : Gamma) (bs : list Binding) :=
+    forall Gamma',
+      (forall x, Term.appears_free_in__bindings_rec x bs -> Gamma x = Gamma' x) ->
+      Delta ,, Gamma' [ flag ]|-oks_r bs.  
+
+  Definition P_binding_well_formed (flag : TypingFlag) (Delta : Delta) (Gamma : Gamma) (b : Binding) :=
+    forall Gamma',
+      (forall x, Term.appears_free_in__binding x b -> Gamma x = Gamma' x) ->
+      Delta ,, Gamma' [ flag ]|-ok_b b.
+
+  #[export] Hint Unfold 
+    P_has_type
+    P_constructor_well_formed
+    P_bindings_well_formed_nonrec
+    P_bindings_well_formed_rec
+    P_binding_well_formed 
+    : core.
+
+  Theorem context_invariance : 
+    (forall flag Delta Gamma t T, Delta ,, Gamma [ flag ]|-+ t : T -> P_has_type flag Delta Gamma t T) /\
+    (forall flag Delta Gamma bs, Delta ,, Gamma [ flag ]|-oks_nr bs -> P_bindings_well_formed_nonrec flag Delta Gamma bs) /\
+    (forall flag Delta Gamma bs, Delta ,, Gamma [ flag ]|-oks_r bs -> P_bindings_well_formed_rec flag Delta Gamma bs) /\
+    (forall flag Delta Gamma b, Delta ,, Gamma [ flag ]|-ok_b b -> P_binding_well_formed flag Delta Gamma b).
+  Proof with eauto.
+    apply has_type__multind with
+      (P := P_has_type)
+      (P0 := P_constructor_well_formed)
+      (P1 := P_bindings_well_formed_nonrec)
+      (P2 := P_bindings_well_formed_rec)
+      (P3 := P_binding_well_formed).
+    all: intros; autounfold; intros.
+    all: try solve [econstructor; eauto].
+
+    - (* T_Var *)
+      eapply T_Var...
+      rewrite <- H1; auto.
+    - (* T_LamAbs *)
+      apply T_LamAbs...
+      apply H2.
       intros.
-      eapply H4.
-      apply AFIT_ExtBuiltin.
-      exists t.
-      split. apply in_combine_l in H5. assumption.
-      auto.
-    + auto.
-  
-  - (* W_Con *)
-    econstructor. eauto.
-    intros.
-    eapply H0.
-    assumption.
-  
-  - (* W_NilB_NonRec *)
-    constructor.
-  - (* W_ConsB_NonRec *)
-    eapply W_ConsB_NonRec.
-    + apply H0.
-      intros.
-      apply H4.
-      apply AFIT_ConsB1_NonRec.
-      assumption.
-    + eassumption.
-    + apply H3.
+      destruct (x =? x0) eqn:Heqb.
+      + apply eqb_eq in Heqb.
+        subst.
+        rewrite update_eq.
+        rewrite update_eq.
+        reflexivity.
+      + apply eqb_neq in Heqb.
+        rewrite update_neq; auto.
+        rewrite update_neq; auto.
+    - (* T_Let *)
+      subst.
+      eapply T_Let...
+      simpl. apply H5.
       intros.
       apply mupdate_eq_cong.
-      apply H4.
-      apply AFIT_ConsB2_NonRec.
-      * unfold P_binding_well_formed in H0.
-        unfold P_bindings_well_formed_nonrec in H2. apply skip. (* TODO *) 
-      * assumption.
-  
-  - (* W_NilB_Rec *)
-    constructor.
-  - (* W_ConsB_Rec *)
-    apply W_ConsB_Rec.
-    + apply H0.
-      intros.
-      apply H3.
-      apply AFIT_ConsB1_Rec.
-      assumption.
-    + apply H2.
-      intros.
-      apply H3.
-      apply AFIT_ConsB2_Rec.
-      assumption.
-  
-  - (* W_Term *)
-    apply W_Term.
-    + assumption.
-    + apply H1.
-      intros.
-      apply H2.
-      apply AFIT_TermBind.
-      assumption.
-  - (* W_Type *)
-    apply W_Type.
-    assumption.
-  - (* W_Data *)
-    subst.
-    eapply W_Data.
-    + reflexivity.
-    + reflexivity.
-    + intros.
-      apply H1.
-      assumption.
-Qed.
+      apply H7.
+      apply Term.AFIT_Let...
+      admit.
 
-    
+    - (* T_LetRec *)
+      subst.
+      eapply T_LetRec...
+      + apply H3.
+        intros.
+        apply mupdate_eq_cong.
+        apply H7.
+        apply Term.AFIT_LetRec...
+        admit.
+      + apply H5.
+        intros.
+        apply mupdate_eq_cong.
+        apply H7.
+        apply Term.AFIT_Let...
+        admit.
+  Admitted.
 
-Lemma free_in_context : forall x t T Delta Gamma,
-    appears_free_in_Term x t ->
-    Delta ,, Gamma |-+ t : T ->
-    exists T', Gamma x = Datatypes.Some T'.
-Proof. Admitted.
-
-Corollary typable_empty__closed_Term : forall t T,
-    empty ,, empty |-+ t : T ->
-    closed_Term t.
-Proof.
-  intros. unfold closed_Term. intros x H1.
-  destruct (free_in_context _ _ _ _ _ H1 H) as [T' C].
-  discriminate C.
-Qed.
-
-Corollary typable_emptyT__closed_Term : forall Delta t T,
-    Delta ,, empty |-+ t : T ->
-    closed_Term t.
-Proof.
-  intros. unfold closed_Term. intros x H1.
-  destruct (free_in_context _ _ _ _ _ H1 H) as [T' C].
-  discriminate C.
-Qed.
-
-
-
-
-
-
-
-Lemma free_in_context_Term : forall x t T Delta Gamma,
-    appears_free_in_Term x t ->
-    Delta ,, Gamma |-+ t : T ->
-    exists T', Gamma x = Datatypes.Some T'.
-Proof.
-  intros x t T Delta Gamma Hafi Htyp.
-  generalize dependent x.
-  induction Htyp.
-  - intros.
-    inversion Hafi.
-    + subst.
-      apply IHHtyp in H8.
-      destruct H8.
-      apply skip.
-    + subst.
-      apply skip.
-  - apply skip.
-  - (* T_Var *)
-    intros.
-    inversion Hafi.
-    subst.
-    exists T. 
-    assumption.
-  - (* T_TyAbs *)
-    intros.
-    inversion Hafi.
-    subst.
-    simpl in IHHtyp.
-    apply IHHtyp.
-    assumption.
-Admitted.
-
-Lemma free_in_context_Annotation : forall X t T Delta Gamma,
-    appears_free_in_Annotation X t ->
-    Delta ,, Gamma |-+ t : T ->
-    exists K, Delta X = Datatypes.Some K.
-Proof.
-  intros x t T Delta Gamma Hafi Htyp.
-  generalize dependent x.
-  induction Htyp.
-  - apply skip.
-  - apply skip.
-  - intros.
-    inversion Hafi. 
-  - intros.
-    inversion Hafi.
-    subst.
-    erewrite <- update_neq; eauto.
-  - intros.
-    inversion Hafi.
-    + subst.
-      eapply free_in_context__Ty; eauto.
-    + subst.
-      simpl in IHHtyp.
-      apply IHHtyp.
-      assumption.
-  - intros. 
-    inversion Hafi. 
-    + subst.
-      apply IHHtyp1.
-      assumption.
-    + subst.
-      apply IHHtyp2.
-      assumption.
-Admitted.
-
-Corollary typable_empty__closed : forall t T,
-    empty ,, empty |-+ t : T ->
-    closed t.
-Proof.
-  intros. unfold closed.
-  split.
-  - intros x H1.
-    destruct (free_in_context_Term _ _ _ _ _ H1 H) as [T' C].
-    discriminate C.
-  - intros X H1.
-    destruct (free_in_context_Annotation _ _ _ _ _ H1 H) as [K C].
-    discriminate C.
-Qed.
+End Typing.
