src/Language/PlutusIR/Semantics/Static/Theorems/ContextInvariance/AFI.v
@@ -4,240 +4,229 @@ Import NamedTerm.
 Require Import Coq.Lists.List.
 Require Import Coq.Strings.String.
 
+Module Ty.
 
+  Inductive appears_free_in : tyname -> Ty -> Prop :=
+    | AFI_TyVar : forall X,
+        appears_free_in X (Ty_Var X)
+    | AFI_TyFun1 : forall X T1 T2,
+        appears_free_in X T1 ->
+        appears_free_in X (Ty_Fun T1 T2)
+    | AFI_TyFun2 : forall X T1 T2,
+        appears_free_in X T2 ->
+        appears_free_in X (Ty_Fun T1 T2)
+    | AFI_TyIFix1 : forall X F T,
+        appears_free_in X F ->
+        appears_free_in X (Ty_IFix F T)
+    | AFI_TyIFix2 : forall X F T,
+        appears_free_in X T ->
+        appears_free_in X (Ty_IFix F T)
+    | AFI_TyForall : forall X bX K T,
+        X <> bX ->
+        appears_free_in X T ->
+        appears_free_in X (Ty_Forall bX K T)
+    | AFI_TyLam : forall X bX K T,
+        X <> bX ->
+        appears_free_in X T ->
+        appears_free_in X (Ty_Lam bX K T)
+    | AFI_TyApp1 : forall X T1 T2,
+        appears_free_in X T1 ->
+        appears_free_in X (Ty_App T1 T2)
+    | AFI_TyApp2 : forall X T1 T2,
+        appears_free_in X T2 ->
+        appears_free_in X (Ty_App T1 T2)
+    .
 
-(** * Free (type) variables and closedness *)
+  Definition closed (T : Ty) :=
+    forall X, ~(appears_free_in X T).
 
-(** ** Types *)
-Inductive appears_free_in_Ty : tyname -> Ty -> Prop :=
-  | AFI_TyVar : forall X,
-      appears_free_in_Ty X (Ty_Var X)
-  | AFI_TyFun1 : forall X T1 T2,
-      appears_free_in_Ty X T1 ->
-      appears_free_in_Ty X (Ty_Fun T1 T2)
-  | AFI_TyFun2 : forall X T1 T2,
-      appears_free_in_Ty X T2 ->
-      appears_free_in_Ty X (Ty_Fun T1 T2)
-  | AFI_TyIFix1 : forall X F T,
-      appears_free_in_Ty X F ->
-      appears_free_in_Ty X (Ty_IFix F T)
-  | AFI_TyIFix2 : forall X F T,
-      appears_free_in_Ty X T ->
-      appears_free_in_Ty X (Ty_IFix F T)
-  | AFI_TyForall : forall X bX K T,
-      X <> bX ->
-      appears_free_in_Ty X T ->
-      appears_free_in_Ty X (Ty_Forall bX K T)
-  | AFI_TyLam : forall X bX K T,
-      X <> bX ->
-      appears_free_in_Ty X T ->
-      appears_free_in_Ty X (Ty_Lam bX K T)
-  | AFI_TyApp1 : forall X T1 T2,
-      appears_free_in_Ty X T1 ->
-      appears_free_in_Ty X (Ty_App T1 T2)
-  | AFI_TyApp2 : forall X T1 T2,
-      appears_free_in_Ty X T2 ->
-      appears_free_in_Ty X (Ty_App T1 T2)
-  .
+End Ty.
+
+Module Term.
+
+  Definition term_var_bound_by_constructor (c : NamedTerm.constructor) : string :=
+    match c with
+    | Constructor (VarDecl x _) _ => x
+    end.
+
+  Definition term_vars_bound_by_binding (b : NamedTerm.Binding) : list string :=
+    match b with
+    | TermBind _ (VarDecl x _) _ => cons x nil
+    | TypeBind (TyVarDecl X _) _ => nil
+    | DatatypeBind (Datatype (TyVarDecl X _) YKs matchFunc cs) => matchFunc :: (rev (map term_var_bound_by_constructor cs))
+    end.
+
+  Definition term_vars_bound_by_bindings (bs : list NamedTerm.Binding) : list string := List.concat (map term_vars_bound_by_binding bs).
+
+  Inductive appears_free_in : name -> Term -> Prop :=
+    | AFIT_Let : forall x r bs t,
+        ~(In x (term_vars_bound_by_bindings bs)) ->
+        appears_free_in x t ->
+        appears_free_in x (Let r bs t)
+    | AFIT_LetNonRec : forall x bs t,
+        appears_free_in__bindings_nonrec x bs ->
+        appears_free_in x (Let NonRec bs t)
+    | AFIT_LetRec : forall x bs t,
+        ~(In x (term_vars_bound_by_bindings bs)) ->
+        appears_free_in__bindings_rec x bs ->
+        appears_free_in x (Let Rec bs t)
+    | AFIT_Var : forall x,
+        appears_free_in x (Var x)
+    | AFIT_TyAbs : forall x bX K t0,
+        appears_free_in x t0 ->
+        appears_free_in x (TyAbs bX K t0)
+    | AFIT_LamAbs : forall x bx T t0,
+        x <> bx ->
+        appears_free_in x t0 ->
+        appears_free_in x (LamAbs bx T t0)
+    | AFIT_Apply1 : forall x t1 t2,
+        appears_free_in x t1 ->
+        appears_free_in x (Apply t1 t2)
+    | AFIT_Apply2 : forall x t1 t2,
+        appears_free_in x t2 ->
+        appears_free_in x (Apply t1 t2)
+    | AFIT_TyInst : forall x t0 T,
+        appears_free_in x t0 ->
+        appears_free_in x (TyInst t0 T)
+    | AFIT_IWrap : forall x F T t0,
+        appears_free_in x t0 ->
+        appears_free_in x (IWrap F T t0)
+    | AFIT_Unwrap : forall x t0,
+        appears_free_in x t0 ->
+        appears_free_in x (Unwrap t0)
+
+  with appears_free_in__bindings_nonrec : name -> list Binding -> Prop :=
+    | AFIT_ConsB1_NonRec : forall x b bs,
+        appears_free_in__binding x b ->
+        appears_free_in__bindings_nonrec x (b :: bs)
+    | AFIT_ConsB2_NonRec : forall x b bs,
+        ~(In x (term_vars_bound_by_binding b)) ->
+        appears_free_in__bindings_nonrec x bs ->
+        appears_free_in__bindings_nonrec x (b :: bs)
+
+  with appears_free_in__bindings_rec : name -> list Binding -> Prop :=
+    | AFIT_ConsB1_Rec : forall x b bs,
+        appears_free_in__binding x b ->
+        appears_free_in__bindings_rec x (b :: bs)
+    | AFIT_ConsB2_Rec : forall x b bs,
+        appears_free_in__bindings_rec x bs ->
+        appears_free_in__bindings_rec x (b :: bs)
+
+  with appears_free_in__binding : name -> Binding -> Prop :=
+    | AFIT_TermBind : forall x s vd t0,
+        appears_free_in x t0 ->
+        appears_free_in__binding x (TermBind s vd t0)
+    .
+
+  Definition closed (t : Term) :=
+    forall x, ~(appears_free_in x t).
+
+End Term.
+
+Module Annotation.
+
+  Definition tyvars_bound_by_binding (b : NamedTerm.Binding) : list tyname :=
+    match b with
+    | TermBind _ (VarDecl x _) _ => nil
+    | TypeBind (TyVarDecl X _) _ => cons X nil
+    | DatatypeBind (Datatype (TyVarDecl X _) YKs matchFunc cs) => cons X nil
+    end.
+
+  Definition tyvars_bound_by_bindings (bs : list NamedTerm.Binding) : list tyname := List.concat (map tyvars_bound_by_binding bs).
+
+  Inductive appears_free_in (X : tyname) : Term -> Prop :=
+    | AFIA_Let : forall r bs t,
+        ~(In X (tyvars_bound_by_bindings bs)) ->
+        appears_free_in X t ->
+        appears_free_in X (Let r bs t)
+    | AFIA_LetNonRec : forall bs t,
+        appears_free_in__bindings_nonrec X bs ->
+        appears_free_in X (Let NonRec bs t)
+    | AFIA_LetRec : forall bs t,
+        ~(In X (tyvars_bound_by_bindings bs)) ->
+        appears_free_in__bindings_rec X bs ->
+        appears_free_in X (Let Rec bs t)
+    | AFIA_TyAbs : forall bX K t0,
+        X <> bX ->
+        appears_free_in X t0 ->
+        appears_free_in X (TyAbs bX K t0)
+    | AFIA_LamAbs1 : forall bx T t0,
+        Ty.appears_free_in X T ->
+        appears_free_in X (LamAbs bx T t0)
+    | AFIA_LamAbs2 : forall bx T t0,
+        appears_free_in X t0 ->
+        appears_free_in X (LamAbs bx T t0)
+    | AFIA_Apply1 : forall t1 t2,
+        appears_free_in X t1 ->
+        appears_free_in X (Apply t1 t2)
+    | AFIA_Apply2 : forall t1 t2,
+        appears_free_in X t2 ->
+        appears_free_in X (Apply t1 t2)
+    | AFIA_TyInst1 : forall t0 T,
+        Ty.appears_free_in X T ->
+        appears_free_in X (TyInst t0 T)
+    | AFIA_TyInst2 : forall t0 T,
+        appears_free_in X t0 ->
+        appears_free_in X (TyInst t0 T)
+    | AFIA_IWrap1 : forall F T t0,
+        Ty.appears_free_in X F ->
+        appears_free_in X (IWrap F T t0)
+    | AFIA_IWrap2 : forall F T t0,
+        Ty.appears_free_in X T ->
+        appears_free_in X (IWrap F T t0)
+    | AFIA_IWrap3 : forall F T t0,
+        appears_free_in X t0 ->
+        appears_free_in X (IWrap F T t0)
+    | AFIA_Unwrap : forall t0,
+        appears_free_in X t0 ->
+        appears_free_in X (Unwrap t0)
+
+  with appears_free_in__constructor (X : tyname) : constructor -> Prop :=
+    (* TODO *)
+
+  with appears_free_in__bindings_nonrec (X : tyname) : list Binding -> Prop :=
+    | AFIA_ConsB1_NonRec : forall b bs,
+        appears_free_in__binding X b ->
+        appears_free_in__bindings_nonrec X (b :: bs)
+    | AFIA_ConsB2_NonRec : forall b bs,
+        ~(In X (tyvars_bound_by_binding b)) ->
+        appears_free_in__bindings_nonrec X bs ->
+        appears_free_in__bindings_nonrec X (b :: bs)
+
+  with appears_free_in__bindings_rec (X : tyname) : list Binding -> Prop :=
+    | AFIA_ConsB1_Rec : forall b bs,
+        appears_free_in__binding X b ->
+        appears_free_in__bindings_rec X (b :: bs)
+    | AFIA_ConsB2_Rec : forall b bs,
+        appears_free_in__bindings_rec X bs ->
+        appears_free_in__bindings_rec X (b :: bs)
+
+  with appears_free_in__binding (X: tyname) : Binding -> Prop :=
+    (* TODO *) .
+
+  Definition closed (t : Term) :=
+    forall x, ~(appears_free_in x t).
+
+End Annotation.
 
 #[export] Hint Constructors 
-  appears_free_in_Ty 
+  Ty.appears_free_in 
   : core.
 
-Definition closed_Ty (T : Ty) :=
-  forall X, ~(appears_free_in_Ty X T).
-
-
-
-(** ** Terms *)
-
-(** *** Utilities *)
-Definition term_var_bound_by_constructor (c : NamedTerm.constructor) : string :=
-  match c with
-  | Constructor (VarDecl x _) _ => x
-  end.
-
-Definition term_vars_bound_by_binding (b : NamedTerm.Binding) : list string :=
-  match b with
-  | TermBind _ (VarDecl x _) _ => cons x nil
-  | TypeBind (TyVarDecl X _) _ => nil
-  | DatatypeBind (Datatype (TyVarDecl X _) YKs matchFunc cs) => matchFunc :: (rev (map term_var_bound_by_constructor cs))
-  end.
-
-Definition term_vars_bound_by_bindings (bs : list NamedTerm.Binding) : list string := List.concat (map term_vars_bound_by_binding bs).
-
-(** *** AFI inductive datatype *)
-Inductive appears_free_in_Term : name -> Term -> Prop :=
-  | AFIT_Let : forall x r bs t,
-      ~(In x (term_vars_bound_by_bindings bs)) ->
-      appears_free_in_Term x t ->
-      appears_free_in_Term x (Let r bs t)
-  | AFIT_LetNonRec : forall x bs t,
-      appears_free_in_Term__bindings_nonrec x bs ->
-      appears_free_in_Term x (Let NonRec bs t)
-  | AFIT_LetRec : forall x bs t,
-      ~(In x (term_vars_bound_by_bindings bs)) ->
-      appears_free_in_Term__bindings_rec x bs ->
-      appears_free_in_Term x (Let Rec bs t)
-  | AFIT_Var : forall x,
-      appears_free_in_Term x (Var x)
-  | AFIT_TyAbs : forall x bX K t0,
-      appears_free_in_Term x t0 ->
-      appears_free_in_Term x (TyAbs bX K t0)
-  | AFIT_LamAbs : forall x bx T t0,
-      x <> bx ->
-      appears_free_in_Term x t0 ->
-      appears_free_in_Term x (LamAbs bx T t0)
-  | AFIT_Apply1 : forall x t1 t2,
-      appears_free_in_Term x t1 ->
-      appears_free_in_Term x (Apply t1 t2)
-  | AFIT_Apply2 : forall x t1 t2,
-      appears_free_in_Term x t2 ->
-      appears_free_in_Term x (Apply t1 t2)
-  | AFIT_TyInst : forall x t0 T,
-      appears_free_in_Term x t0 ->
-      appears_free_in_Term x (TyInst t0 T)
-  | AFIT_IWrap : forall x F T t0,
-      appears_free_in_Term x t0 ->
-      appears_free_in_Term x (IWrap F T t0)
-  | AFIT_Unwrap : forall x t0,
-      appears_free_in_Term x t0 ->
-      appears_free_in_Term x (Unwrap t0)
-  | AFIT_ExtBuiltin : forall x f args,
-      (exists arg, In arg args /\ appears_free_in_Term x arg) ->
-      appears_free_in_Term x (ExtBuiltin f args)
-
-with appears_free_in_Term__bindings_nonrec : name -> list Binding -> Prop :=
-  | AFIT_ConsB1_NonRec : forall x b bs,
-      appears_free_in_Term__binding x b ->
-      appears_free_in_Term__bindings_nonrec x (b :: bs)
-  | AFIT_ConsB2_NonRec : forall x b bs,
-      ~(In x (term_vars_bound_by_binding b)) ->
-      appears_free_in_Term__bindings_nonrec x bs ->
-      appears_free_in_Term__bindings_nonrec x (b :: bs)
-
-with appears_free_in_Term__bindings_rec : name -> list Binding -> Prop :=
-  | AFIT_ConsB1_Rec : forall x b bs,
-      appears_free_in_Term__binding x b ->
-      appears_free_in_Term__bindings_rec x (b :: bs)
-  | AFIT_ConsB2_Rec : forall x b bs,
-      appears_free_in_Term__bindings_rec x bs ->
-      appears_free_in_Term__bindings_rec x (b :: bs)
-
-with appears_free_in_Term__binding : name -> Binding -> Prop :=
-  | AFIT_TermBind : forall x s vd t0,
-      appears_free_in_Term x t0 ->
-      appears_free_in_Term__binding x (TermBind s vd t0)
-  .
-
 #[export] Hint Constructors 
-  appears_free_in_Term 
-  appears_free_in_Term__bindings_nonrec
-  appears_free_in_Term__bindings_rec
-  appears_free_in_Term__binding 
+  Term.appears_free_in 
+  Term.appears_free_in__bindings_nonrec
+  Term.appears_free_in__bindings_rec
+  Term.appears_free_in__binding 
   : core.
 
-(** *** Closedness of Terms *)
-Definition closed_Term (t : Term) :=
-  forall x, ~(appears_free_in_Term x t).
-
-
-
-(** ** Type annotations *)
-Definition tyvars_bound_by_binding (b : NamedTerm.Binding) : list tyname :=
-  match b with
-  | TermBind _ (VarDecl x _) _ => nil
-  | TypeBind (TyVarDecl X _) _ => cons X nil
-  | DatatypeBind (Datatype (TyVarDecl X _) YKs matchFunc cs) => cons X nil
-  end.
-
-Definition tyvars_bound_by_bindings (bs : list NamedTerm.Binding) : list tyname := List.concat (map tyvars_bound_by_binding bs).
-
-
-(** *** AFIA inductive datatype *)
-Inductive appears_free_in_Annotation (X : tyname) : Term -> Prop :=
-  | AFIA_Let : forall r bs t,
-      ~(In X (tyvars_bound_by_bindings bs)) ->
-      appears_free_in_Annotation X t ->
-      appears_free_in_Annotation X (Let r bs t)
-  | AFIA_LetNonRec : forall bs t,
-      appears_free_in_Annotation__bindings_nonrec X bs ->
-      appears_free_in_Annotation X (Let NonRec bs t)
-  | AFIA_LetRec : forall bs t,
-      ~(In X (tyvars_bound_by_bindings bs)) ->
-      appears_free_in_Annotation__bindings_rec X bs ->
-      appears_free_in_Annotation X (Let Rec bs t)
-  | AFIA_TyAbs : forall bX K t0,
-      X <> bX ->
-      appears_free_in_Annotation X t0 ->
-      appears_free_in_Annotation X (TyAbs bX K t0)
-  | AFIA_LamAbs1 : forall bx T t0,
-      appears_free_in_Ty X T ->
-      appears_free_in_Annotation X (LamAbs bx T t0)
-  | AFIA_LamAbs2 : forall bx T t0,
-      appears_free_in_Annotation X t0 ->
-      appears_free_in_Annotation X (LamAbs bx T t0)
-  | AFIA_Apply1 : forall t1 t2,
-      appears_free_in_Annotation X t1 ->
-      appears_free_in_Annotation X (Apply t1 t2)
-  | AFIA_Apply2 : forall t1 t2,
-      appears_free_in_Annotation X t2 ->
-      appears_free_in_Annotation X (Apply t1 t2)
-  | AFIA_TyInst1 : forall t0 T,
-      appears_free_in_Ty X T ->
-      appears_free_in_Annotation X (TyInst t0 T)
-  | AFIA_TyInst2 : forall t0 T,
-      appears_free_in_Annotation X t0 ->
-      appears_free_in_Annotation X (TyInst t0 T)
-  | AFIA_Error : forall T,
-      appears_free_in_Ty X T ->
-      appears_free_in_Annotation X (Error T)
-  | AFIA_IWrap1 : forall F T t0,
-      appears_free_in_Ty X F ->
-      appears_free_in_Annotation X (IWrap F T t0)
-  | AFIA_IWrap2 : forall F T t0,
-      appears_free_in_Ty X T ->
-      appears_free_in_Annotation X (IWrap F T t0)
-  | AFIA_IWrap3 : forall F T t0,
-      appears_free_in_Annotation X t0 ->
-      appears_free_in_Annotation X (IWrap F T t0)
-  | AFIA_Unwrap : forall t0,
-      appears_free_in_Annotation X t0 ->
-      appears_free_in_Annotation X (Unwrap t0)
-
-with appears_free_in_Annotation__bindings_nonrec (X : tyname) : list Binding -> Prop :=
-  | AFIA_ConsB1_NonRec : forall b bs,
-      appears_free_in_Annotation__binding X b ->
-      appears_free_in_Annotation__bindings_nonrec X (b :: bs)
-  | AFIA_ConsB2_NonRec : forall b bs,
-      ~(In X (tyvars_bound_by_binding b)) ->
-      appears_free_in_Annotation__bindings_nonrec X bs ->
-      appears_free_in_Annotation__bindings_nonrec X (b :: bs)
-
-with appears_free_in_Annotation__bindings_rec (X : tyname) : list Binding -> Prop :=
-  | AFIA_ConsB1_Rec : forall b bs,
-      appears_free_in_Annotation__binding X b ->
-      appears_free_in_Annotation__bindings_rec X (b :: bs)
-  | AFIA_ConsB2_Rec : forall b bs,
-      appears_free_in_Annotation__bindings_rec X bs ->
-      appears_free_in_Annotation__bindings_rec X (b :: bs)
-
-with appears_free_in_Annotation__binding (X: tyname) : Binding -> Prop :=
-  (* TODO *) .
-
-
 #[export] Hint Constructors 
-  appears_free_in_Annotation 
-  appears_free_in_Annotation__bindings_nonrec
-  appears_free_in_Annotation__bindings_rec
-  appears_free_in_Annotation__binding : core. 
+  Annotation.appears_free_in 
+  Annotation.appears_free_in__constructor
+  Annotation.appears_free_in__bindings_nonrec
+  Annotation.appears_free_in__bindings_rec
+  Annotation.appears_free_in__binding : core. 
 
-(** *** Closedness of type annotations *)
-Definition closed_Annotation (t : Term) :=
-  forall x, ~(appears_free_in_Term x t).
-
-
-
-(** * Full closedness of terms (and type annotations) *)
+(** Full closedness of terms (and type annotations) *)
 Definition closed (t : Term) :=
-  (forall x, ~(appears_free_in_Term x t)) /\ (forall X, ~(appears_free_in_Annotation X t)).
+  (forall x, ~(Term.appears_free_in x t)) /\ (forall X, ~(Annotation.appears_free_in X t)).
