src/Language/PlutusIR/Semantics/Static/Theorems/Weakening.v
@@ -1,131 +1,104 @@
 Require Import PlutusCert.Language.PlutusIR.
 Import NamedTerm.
+
 Require Import PlutusCert.Language.PlutusIR.Semantics.Static.Rules.
-
-Import Coq.Strings.String.
-Local Open Scope string_scope.
       
-Lemma weakening__has_kind : forall Delta Delta' T K,
-    inclusion Delta Delta' ->
-    Delta |-* T : K ->
-    Delta' |-* T : K.
-Proof.
-  intros Delta Delta' T K H HT.
-  generalize dependent Delta'.
-  induction HT; intros; eauto using inclusion_update with typing.
-Qed.
+Module Kinding.
 
-Lemma weakening_empty__has_kind : forall Delta T K,
-    empty |-* T : K ->
-    Delta |-* T : K.
-Proof.
-  intros.
-  eapply weakening__has_kind; eauto using inclusion_empty.
-Qed.
+  Lemma weakening : forall Delta Delta' T K,
+      inclusion Delta Delta' ->
+      Delta |-* T : K ->
+      Delta' |-* T : K.
+  Proof.
+    intros Delta Delta' T K H HT.
+    generalize dependent Delta'.
+    induction HT.
+    all: intros Delta' Hincl.
+    all: try solve [econstructor; eauto using inclusion_update].
+  Qed.
 
-
-Definition P_has_type Delta Gamma t T : Prop :=
-  forall Delta' Gamma',
-    inclusion Delta Delta' ->
-    inclusion Gamma Gamma' ->
-    Delta' ,, Gamma' |-+ t : T.
-
-Definition P_constructor_well_formed Delta c : Prop :=
-  forall Delta',
-    inclusion Delta Delta' ->
-    Delta' |-ok_c c.
-
-Definition P_bindings_well_formed_nonrec Delta Gamma bs : Prop :=
-  forall Delta' Gamma',
-    inclusion Delta Delta' ->
-    inclusion Gamma Gamma' ->
-    Delta' ,, Gamma' |-oks_nr bs.
-
-Definition P_bindings_well_formed_rec Delta Gamma bs : Prop :=
-  forall Delta' Gamma',
-    inclusion Delta Delta' ->
-    inclusion Gamma Gamma' ->
-    Delta' ,, Gamma' |-oks_r bs.
-
-Definition P_binding_well_formed Delta Gamma b : Prop :=
-  forall Delta' Gamma',
-    inclusion Delta Delta' ->
-    inclusion Gamma Gamma' ->
-    Delta' ,, Gamma' |-ok b.
-
-#[export] Hint Unfold
-  P_has_type
-  P_constructor_well_formed
-  P_bindings_well_formed_nonrec
-  P_bindings_well_formed_rec
-  P_binding_well_formed 
-  : core.
-
-Lemma weakening : 
-  (forall Delta Gamma t T, Delta ,, Gamma |-+ t : T -> P_has_type Delta Gamma t T) /\
-  (forall Delta Gamma bs, Delta ,, Gamma |-oks_nr bs -> P_bindings_well_formed_nonrec Delta Gamma bs) /\
-  (forall Delta Gamma bs, Delta ,, Gamma |-oks_r bs -> P_bindings_well_formed_rec Delta Gamma bs) /\
-  (forall Delta Gamma b, Delta ,, Gamma |-ok b -> P_binding_well_formed Delta Gamma b).
-Proof with eauto using weakening__has_kind, inclusion_update with typing.
-  apply has_type__multind with 
-    (P := P_has_type) 
-    (P0 := P_constructor_well_formed)
-    (P1 := P_bindings_well_formed_nonrec)
-    (P2 := P_bindings_well_formed_rec)
-    (P3 := P_binding_well_formed).
-  all: intros; autounfold; intros...
-  - (* T_Let *)
-    subst.
-    eapply T_Let...
-    + apply H5.
-      * apply inclusion_mupdate.
-        assumption.
-      * apply inclusion_mupdate.
-        assumption.
-  - (* T_LetRec *)
-    subst.
-    eapply T_LetRec...
-    + apply H3.
-      * apply inclusion_mupdate.
-        assumption.
-      * apply inclusion_mupdate.
-        assumption.
-    + apply H5.
-      * apply inclusion_mupdate.
-        assumption.
-      * apply inclusion_mupdate.
-        assumption.
-  - (* T_ExtBuiltin *)
-    eapply T_ExtBuiltin; eauto.
+  Lemma weakening_empty : forall Delta T K,
+      empty |-* T : K ->
+      Delta |-* T : K.
+  Proof.
     intros.
-    eapply H2; eauto.
-  - (* W_ConsB_NonRec *)
-    eapply W_ConsB_NonRec...
-    + apply H3.
-      apply inclusion_mupdate.
-      assumption.
-      apply inclusion_mupdate.
-      assumption.
-  - (* W_Data *)
-    eapply W_Data.
-    + reflexivity.
-    + reflexivity.
-    + intros.
-      apply H2.
-      * assumption.
-      * subst.
-        apply inclusion_mupdate.
-        assumption.
-Qed.
+    eapply weakening; eauto using inclusion_empty.
+  Qed.
 
-Lemma weakening_empty : forall Delta Gamma t T,
-    empty ,, empty |-+ t : T ->
-    Delta ,, Gamma |-+ t : T.
-Proof.
-  intros Delta Gamma t T Ht.
-  apply weakening in Ht.
-  unfold P_has_type in Ht.
-  apply Ht.
-  - apply inclusion_empty.
-  - apply inclusion_empty.
-Qed.
+End Kinding.
+
+Module Typing.
+
+  Definition P_has_type flag Delta Gamma t T : Prop :=
+    forall Delta' Gamma',
+      inclusion Delta Delta' ->
+      inclusion Gamma Gamma' ->
+      Delta' ,, Gamma' [ flag ]|-+ t : T.
+
+  Definition P_constructor_well_formed Delta c T : Prop :=
+    forall Delta',
+      inclusion Delta Delta' ->
+      Delta' |-ok_c c : T.
+
+  Definition P_bindings_well_formed_nonrec flag Delta Gamma bs : Prop :=
+    forall Delta' Gamma',
+      inclusion Delta Delta' ->
+      inclusion Gamma Gamma' ->
+      Delta' ,, Gamma' [ flag ]|-oks_nr bs.
+
+  Definition P_bindings_well_formed_rec flag Delta Gamma bs : Prop :=
+    forall Delta' Gamma',
+      inclusion Delta Delta' ->
+      inclusion Gamma Gamma' ->
+      Delta' ,, Gamma' [ flag ]|-oks_r bs.
+
+  Definition P_binding_well_formed flag Delta Gamma b : Prop :=
+    forall Delta' Gamma',
+      inclusion Delta Delta' ->
+      inclusion Gamma Gamma' ->
+      Delta' ,, Gamma' [ flag ]|-ok_b b.
+
+  #[export] Hint Unfold
+    P_has_type
+    P_constructor_well_formed
+    P_bindings_well_formed_nonrec
+    P_bindings_well_formed_rec
+    P_binding_well_formed 
+    : core.
+
+  Lemma weakening : 
+    (forall flag Delta Gamma t T, Delta ,, Gamma [ flag ]|-+ t : T -> P_has_type flag Delta Gamma t T) /\
+    (forall flag Delta Gamma bs, Delta ,, Gamma [ flag ]|-oks_nr bs -> P_bindings_well_formed_nonrec flag Delta Gamma bs) /\
+    (forall flag Delta Gamma bs, Delta ,, Gamma [ flag ]|-oks_r bs -> P_bindings_well_formed_rec flag Delta Gamma bs) /\
+    (forall flag Delta Gamma b, Delta ,, Gamma [ flag ]|-ok_b b -> P_binding_well_formed flag Delta Gamma b).
+  Proof with eauto using Kinding.weakening, inclusion_update, inclusion_mupdate.
+    apply has_type__multind with 
+      (P := P_has_type) 
+      (P0 := P_constructor_well_formed)
+      (P1 := P_bindings_well_formed_nonrec)
+      (P2 := P_bindings_well_formed_rec)
+      (P3 := P_binding_well_formed).
+    all: intros; autounfold.
+    all: try (intros Delta'_0 Gamma'_0 HinclD HinclG).
+    all: try (intros Delta'_0 HinclD).
+    all: try solve [econstructor; subst; eauto using Kinding.weakening, inclusion_update, inclusion_mupdate].
+    - (* W_Con *)
+      econstructor...
+      subst.
+      intros.
+      eapply H1...
+  Qed.
+
+  Lemma weakening_empty : forall flag Delta Gamma t T,
+      empty ,, empty [ flag ]|-+ t : T ->
+      Delta ,, Gamma [ flag ]|-+ t : T.
+  Proof.
+    intros flag Delta Gamma t T Ht.
+    apply weakening in Ht.
+    unfold P_has_type in Ht.
+    apply Ht.
+    - apply inclusion_empty.
+    - apply inclusion_empty.
+  Qed.
+
+End Typing.
