src/Language/PlutusIR/Semantics/Static/TypeSubstitution.v
@@ -5,9 +5,8 @@ Require Import Coq.Lists.List.
 Require Import Coq.Strings.String.
 Local Open Scope string_scope.
 
-(** * Substitution of types *)
+(** * Regular substitution of types *)
 
-(** ** Implementation as a fixpoint *)
 Fixpoint substituteT (X : tyname) (S T : Ty) : Ty :=
   match T with
   | Ty_Var Y => 
@@ -26,14 +25,103 @@ Fixpoint substituteT (X : tyname) (S T : Ty) : Ty :=
     Ty_App (substituteT X S T1) (substituteT X S T2)
   end.
 
+(** Multi-substitutions of types*)
+Definition envT := list (tyname * Ty).
 
-
-(** * Multi-substitutions of types*)
-
-Definition env := list (tyname * Ty).
-
-Fixpoint msubstT (ss : env) (T : Ty) : Ty :=
+Fixpoint msubstT (ss : envT) (T : Ty) : Ty :=
   match ss with
   | nil => T
   | (a, T0) :: ss' => msubstT ss' (substituteT a T0 T)
   end.
+
+(** * Capture-avoiding substitution of types *)
+Require Import PlutusCert.Language.PlutusIR.Semantics.Static.Theorems.ContextInvariance.AFI.
+Require Import Lia.
+Import ListNotations.
+
+Fixpoint ftv (T : Ty) : list tyname :=
+  match T with
+  | Ty_Var X => 
+      [X]
+  | Ty_Fun T1 T2 =>
+      ftv T1 ++ ftv T2
+  | Ty_IFix F T =>
+      ftv F ++ ftv T
+  | Ty_Forall X K T' =>
+      remove string_dec X (ftv T')
+  | Ty_Builtin u => 
+      []
+  | Ty_Lam X K1 T' =>
+      remove string_dec X (ftv T')
+  | Ty_App T1 T2 =>
+      ftv T1 ++ ftv T2
+  end.
+
+(* TODO: Actually generate a fresh type variable *)
+Definition fresh (T : Ty) (X : tyname) : tyname := "a".
+
+Definition rename (X Y : tyname) (T : Ty) := substituteT X (Ty_Var Y) T.
+
+Fixpoint size (T : Ty) : nat := 
+  match T with
+  | Ty_Var Y => 1
+  | Ty_Fun T1 T2 => 1 + size T1 + size T2
+  | Ty_IFix F T => 1 + size F + size T  
+  | Ty_Forall bX K T0 => 1 + size T0
+  | Ty_Builtin u => 1
+  | Ty_Lam bX K T0 => 1 + size T0
+  | Ty_App T1 T2 => 1 + size T1 + size T2 
+  end.
+
+Lemma rename_preserves_size : forall T X Y,
+    size T = size (rename X Y T).
+Proof.
+  unfold rename.
+  induction T; intros; simpl; eauto.
+  - destruct (X =? t); eauto.
+  - destruct (X =? b); simpl; eauto.
+  - destruct (X =? b); simpl; eauto.
+Qed.
+
+Equations? substituteTCA (X : tyname) (U T : Ty) : Ty by wf (size T) :=
+  substituteTCA X U (Ty_Var Y) => 
+      if X =? Y then U else Ty_Var Y ;
+  substituteTCA X U (Ty_Fun T1 T2) =>
+      Ty_Fun (substituteTCA X U T1) (substituteTCA X U T2) ;
+  substituteTCA X U (Ty_IFix F T) =>
+      Ty_IFix (substituteTCA X U F) (substituteTCA X U T) ;
+  substituteTCA X U (Ty_Forall Y K T0) =>
+      if X =? Y 
+        then 
+          Ty_Forall Y K T0
+        else 
+          if existsb (eqb Y) (ftv U) 
+            then 
+              let Y' := fresh U Y in
+              let T0' := rename Y Y' T0 in
+              Ty_Forall Y' K (substituteTCA X U T0')
+            else
+              Ty_Forall Y K T0 ;
+  substituteTCA X U (Ty_Builtin u) =>
+      Ty_Builtin u ;
+  substituteTCA X U (Ty_Lam Y K T0) =>
+      if X =? Y 
+        then 
+          Ty_Lam Y K T0 
+        else 
+          if existsb (eqb Y) (ftv U) 
+            then 
+              let Y' := fresh U Y in
+              let T0' := rename Y Y' T0 in
+              Ty_Lam Y' K (substituteTCA X U T0') 
+            else
+              Ty_Lam Y K (substituteTCA X U T0) ;
+  substituteTCA X U (Ty_App T1 T2) => 
+      Ty_App (substituteTCA X U T1) (substituteTCA X U T2)
+  .
+Proof. 
+  all: try solve 
+    [ lia 
+    || replace T0' with (rename Y Y' T0); eauto; rewrite <- rename_preserves_size; eauto
+    ].
+Qed.
