src/Language/PlutusIR/Semantics/Static.v
@@ -2,12 +2,20 @@
 Require Export PlutusCert.Language.PlutusIR.Semantics.Static.Implementations.
 Require Export PlutusCert.Language.PlutusIR.Semantics.Static.Rules.
 Require Export PlutusCert.Language.PlutusIR.Semantics.Static.TypeSubstitution.
-Require Export PlutusCert.Language.PlutusIR.Semantics.Static.TypeSubstitution.CaptureAvoiding.
 Require Export PlutusCert.Language.PlutusIR.Semantics.Static.Normalisation.
 
 (** Important theorems *)
 Require Export PlutusCert.Language.PlutusIR.Semantics.Static.Theorems.ContextInvariance.
 Require Export PlutusCert.Language.PlutusIR.Semantics.Static.Theorems.ContextInvariance.AFI.
+Require Export PlutusCert.Language.PlutusIR.Semantics.Static.Theorems.FreeInContext.
 Require Export PlutusCert.Language.PlutusIR.Semantics.Static.Theorems.UniqueTypes.
 Require Export PlutusCert.Language.PlutusIR.Semantics.Static.Theorems.Weakening.
-Require Export PlutusCert.Language.PlutusIR.Semantics.Static.TypeSubstitution.Equivalence.
+
+(** Hint database *)
+Create HintDb typing.
+#[export] Hint Constructors has_kind : typing.
+#[export] Hint Constructors has_type : typing.
+#[export] Hint Constructors constructor_well_formed : typing.
+#[export] Hint Constructors bindings_well_formed_nonrec : typing.
+#[export] Hint Constructors bindings_well_formed_rec : typing.
+#[export] Hint Constructors binding_well_formed : typing.
