src/Language/PlutusIR/Semantics/Static/Kinding.v
@@ -1,0 +1,44 @@
+Require Import PlutusCert.Language.PlutusIR.
+Import NamedTerm.
+
+Require Export PlutusCert.Language.PlutusIR.Semantics.Static.Context.
+
+(** Kinds of built-in types *)
+Definition lookupBuiltinKind (u : DefaultUni) : Kind := 
+  match u with
+  | DefaultUniInteger    => Kind_Base
+  | DefaultUniByteString => Kind_Base
+  | DefaultUniString     => Kind_Base
+  | DefaultUniChar       => Kind_Base
+  | DefaultUniUnit       => Kind_Base
+  | DefaultUniBool       => Kind_Base
+  end.
+
+(** Kinding of types *)
+Reserved Notation "Delta '|-*' T ':' K" (at level 40, T at level 0, K at level 0).
+Inductive has_kind : Delta -> Ty -> Kind -> Prop :=
+  | K_Var : forall Delta X K,
+      Delta X = Coq.Init.Datatypes.Some K ->
+      Delta |-* (Ty_Var X) : K
+  | K_Fun : forall Delta T1 T2,
+      Delta |-* T1 : Kind_Base ->
+      Delta |-* T2 : Kind_Base ->
+      Delta |-* (Ty_Fun T1 T2) : Kind_Base
+  | K_IFix  : forall Delta F T K,
+      Delta |-* T : K ->
+      Delta |-* F : (Kind_Arrow (Kind_Arrow K Kind_Base) (Kind_Arrow K Kind_Base)) ->
+      Delta |-* (Ty_IFix F T) : Kind_Base
+  | K_Forall : forall Delta X K T,
+      (X |-> K; Delta) |-* T : Kind_Base ->
+      Delta |-* (Ty_Forall X K T) : Kind_Base
+  | K_Builtin : forall Delta u T,
+      T = lookupBuiltinKind u ->
+      Delta |-* (Ty_Builtin (Some (TypeIn u))) : T
+  | K_Lam : forall Delta X K1 T K2,
+      (X |-> K1; Delta) |-* T : K2 ->
+      Delta |-* (Ty_Lam X K1 T) : (Kind_Arrow K1 K2)
+  | K_App : forall Delta T1 T2 K1 K2,
+      Delta |-* T1 : (Kind_Arrow K1 K2) ->
+      Delta |-* T2 : K1 ->
+      Delta |-* (Ty_App T1 T2) : K2
+where "Delta '|-*' T ':' K" := (has_kind Delta T K).
