src/Language/PlutusIR/Semantics/Static/Theorems/FreeInContext.v
@@ -1,0 +1,189 @@
+Require Import PlutusCert.Language.PlutusIR.
+Import NamedTerm.
+
+Require Import PlutusCert.Language.PlutusIR.Semantics.Static.Theorems.ContextInvariance.AFI.
+Require Import PlutusCert.Language.PlutusIR.Semantics.Static.Rules.
+
+Module Ty.
+
+  Lemma free_in_context : forall Delta T K,
+    Delta |-* T : K ->
+    forall X,
+      Ty.appears_free_in X T ->
+      exists K', Delta X = Datatypes.Some K'.
+  Proof with eauto.
+    induction 1.
+    all: intros X0 Hafi.
+    all: try solve [inversion Hafi; subst; eauto].
+    - inversion Hafi. subst.
+      eapply IHhas_kind in H5.
+      rewrite update_neq in H5...
+    - inversion Hafi. subst.
+      eapply IHhas_kind in H5.
+      rewrite update_neq in H5...
+  Qed.
+
+End Ty.
+
+Module Term.
+
+  Definition P_has_type (flag : TypingFlag) (Delta : Delta) (Gamma : Gamma) (t : Term) (T : Ty) :=
+    forall x,
+      Term.appears_free_in x t ->
+      exists T', Gamma x = Datatypes.Some T'.
+      
+  Definition P_constructor_well_formed (Delta : Delta) (c : constructor) (T : Ty) :=
+    Delta |-ok_c c : T.
+
+  Definition P_bindings_well_formed_nonrec (flag : TypingFlag) (Delta : Delta) (Gamma : Gamma) (bs : list Binding) :=
+    forall x,
+      Term.appears_free_in__bindings_nonrec x bs ->
+      exists T', Gamma x = Datatypes.Some T'.
+
+  Definition P_bindings_well_formed_rec (flag : TypingFlag) (Delta : Delta) (Gamma : Gamma) (bs : list Binding) :=
+    forall x,
+      Term.appears_free_in__bindings_rec x bs ->
+      exists T', Gamma x = Datatypes.Some T'.
+
+  Definition P_binding_well_formed (flag : TypingFlag) (Delta : Delta) (Gamma : Gamma) (b : Binding) :=
+    forall x,
+      Term.appears_free_in__binding x b ->
+      exists T', Gamma x = Datatypes.Some T'.
+
+  #[export] Hint Unfold
+    P_has_type
+    P_constructor_well_formed
+    P_bindings_well_formed_nonrec
+    P_bindings_well_formed_rec
+    P_binding_well_formed
+    : core.
+
+  Lemma free_in_context :
+      (forall flag Delta Gamma t T, Delta ,, Gamma [ flag ]|-+ t : T -> P_has_type flag Delta Gamma t T) /\
+      (forall flag Delta Gamma bs, Delta ,, Gamma [ flag ]|-oks_nr bs -> P_bindings_well_formed_nonrec flag Delta Gamma bs) /\
+      (forall flag Delta Gamma bs, Delta ,, Gamma [ flag ]|-oks_r bs -> P_bindings_well_formed_rec flag Delta Gamma bs) /\
+      (forall flag Delta Gamma b, Delta ,, Gamma [ flag ]|-ok_b b -> P_binding_well_formed flag Delta Gamma b).
+  Proof with eauto.
+    apply has_type__multind with
+      (P := P_has_type)
+      (P0 := P_constructor_well_formed)
+      (P1 := P_bindings_well_formed_nonrec)
+      (P2 := P_bindings_well_formed_rec)
+      (P3 := P_binding_well_formed).
+    all: intros; autounfold.
+    all: try solve [econstructor; eauto].
+    all: try (intros x0 Hafi).
+    all: try solve [inversion Hafi; subst; eauto].
+    - (* T_LamAbs *)
+      inversion Hafi. subst.
+      eapply H2 in H8...
+      rewrite update_neq in H8...
+    - (* T_Let *)
+      inversion Hafi.
+      + subst.
+        eapply H5 in H12...
+        admit.
+      + subst.
+        eapply H3 in H9...
+    - (* T_LetRec *)
+      inversion Hafi.
+      + subst.
+        eapply H5 in H12...
+        admit.
+      + subst.
+        eapply H3 in H11...
+        admit.
+  Admitted.
+
+End Term.
+
+Module Annotation.
+
+  Definition P_has_type (flag : TypingFlag) (Delta : Delta) (Gamma : Gamma) (t : Term) (T : Ty) :=
+    forall X,
+      Annotation.appears_free_in X t ->
+      exists K', Delta X = Datatypes.Some K'.
+      
+  Definition P_constructor_well_formed (Delta : Delta) (c : constructor) (T : Ty) :=
+    forall X,
+      Annotation.appears_free_in__constructor X c ->
+      exists K', Delta X = Datatypes.Some K'.
+
+  Definition P_bindings_well_formed_nonrec (flag : TypingFlag) (Delta : Delta) (Gamma : Gamma) (bs : list Binding) :=
+    forall X,
+      Annotation.appears_free_in__bindings_nonrec X bs ->
+      exists K', Delta X = Datatypes.Some K'.
+
+  Definition P_bindings_well_formed_rec (flag : TypingFlag) (Delta : Delta) (Gamma : Gamma) (bs : list Binding) :=
+    forall X,
+      Annotation.appears_free_in__bindings_rec X bs ->
+      exists K', Delta X = Datatypes.Some K'.
+
+  Definition P_binding_well_formed (flag : TypingFlag) (Delta : Delta) (Gamma : Gamma) (b : Binding) :=
+    forall X,
+      Annotation.appears_free_in__binding X b ->
+      exists K', Delta X = Datatypes.Some K'.
+
+    
+  #[export] Hint Unfold
+    P_has_type
+    P_constructor_well_formed
+    P_bindings_well_formed_nonrec
+    P_bindings_well_formed_rec
+    P_binding_well_formed
+    : core.
+
+  Lemma free_in_context : 
+      (forall flag Delta Gamma t T, Delta ,, Gamma [ flag ]|-+ t : T -> P_has_type flag Delta Gamma t T) /\
+      (forall flag Delta Gamma bs, Delta ,, Gamma [ flag ]|-oks_nr bs -> P_bindings_well_formed_nonrec flag Delta Gamma bs) /\
+      (forall flag Delta Gamma bs, Delta ,, Gamma [ flag ]|-oks_r bs -> P_bindings_well_formed_rec flag Delta Gamma bs) /\
+      (forall flag Delta Gamma b, Delta ,, Gamma [ flag ]|-ok_b b -> P_binding_well_formed flag Delta Gamma b).
+  Proof with (eauto using Ty.free_in_context).
+    apply has_type__multind with
+      (P := P_has_type)
+      (P0 := P_constructor_well_formed)
+      (P1 := P_bindings_well_formed_nonrec)
+      (P2 := P_bindings_well_formed_rec)
+      (P3 := P_binding_well_formed).
+    all: intros; autounfold.
+    all: try (intros x0 Hafi).
+    all: try solve [inversion Hafi; subst; eauto using Ty.free_in_context].
+    - (* T_TyAbs *)
+      inversion Hafi.
+      subst.
+      eapply H0 in H5...
+      rewrite update_neq in H5...
+    - (* T_Let*)
+      inversion Hafi.
+      + subst.
+        eapply H5 in H11...
+        admit.
+      + subst.
+        eapply H3 in H8...
+    - (* T_LetRec *)
+      inversion Hafi.
+      + subst.
+        eapply H5 in H11...
+        admit.
+      + subst.
+        eapply H3 in H10...
+        admit.
+  Admitted.
+
+End Annotation.
+
+Corollary typable_empty__closed : forall flag t T,
+    empty ,, empty [ flag ]|-+ t : T ->
+    closed t.
+Proof with eauto.
+  intros. unfold closed.
+  split.
+  - intros x H1.
+    eapply Term.free_in_context in H1...
+    destruct H1 as [T' C]...
+    discriminate C.
+  - intros X H1.
+    eapply Annotation.free_in_context in H1...
+    destruct H1 as [K' C]...
+    discriminate C.
+Qed.
